

De Morgan:  $\neg(p \wedge q) \vdash (\neg p \vee \neg q)$ . Proof:

|    |                                |                        |
|----|--------------------------------|------------------------|
| 1  | $\neg(p \wedge q)$             |                        |
| 2  | $\neg(\neg p \vee \neg q)$     |                        |
| 3  | $\neg p$                       |                        |
| 4  | $(\neg p \vee \neg q)$         | $\vee I \quad 6$       |
| 5  | $\perp$                        | $\perp I \quad 3, 8$   |
| 6  | $\neg\neg p$                   | $\neg I \quad 3 - 9$   |
| 7  | $p$                            | $\neg E \quad 11$      |
| 8  | $\neg q$                       |                        |
| 9  | $(\neg p \vee \neg q)$         | $\vee I \quad 14$      |
| 10 | $\perp$                        | $\perp I \quad 3, 16$  |
| 11 | $\neg\neg q$                   | $\neg I \quad 14 - 17$ |
| 12 | $q$                            | $\neg E \quad 11$      |
| 13 | $(p \wedge q)$                 | $\wedge I \quad 7, 12$ |
| 14 | $\perp$                        | $\perp I \quad 1, 13$  |
| 15 | $\neg\neg(\neg p \vee \neg q)$ | $\neg I \quad 2, 14$   |
| 16 | $(\neg p \vee \neg q)$         | $\neg E \quad 15$      |